feat: mutual recursive characterization of IsDefEq

Lean4Lean/Theory/Typing/Strong.lean
@@ -37,12 +37,15 @@ inductive IsDefEqStrong : List VExpr → VExpr → VExpr → VExpr → Prop wher
     u.WF uvars → v.WF uvars →
     Γ ⊢ A ≡ A' : .sort u →
     A::Γ ⊢ B : .sort v →
+    A'::Γ ⊢ B : .sort v →
     A::Γ ⊢ body ≡ body' : B →
+    A'::Γ ⊢ body ≡ body' : B →
     Γ ⊢ .lam A body ≡ .lam A' body' : .forallE A B
   | forallEDF :
     u.WF uvars → v.WF uvars →
     Γ ⊢ A ≡ A' : .sort u →
     A::Γ ⊢ body ≡ body' : .sort v →
+    A'::Γ ⊢ body ≡ body' : .sort v →
     Γ ⊢ .forallE A body ≡ .forallE A' body' : .sort (.imax u v)
   | defeqDF :
     u.WF uvars → Γ ⊢ A ≡ B : .sort u → Γ ⊢ e1 ≡ e2 : A → Γ ⊢ e1 ≡ e2 : B
@@ -53,8 +56,12 @@ inductive IsDefEqStrong : List VExpr → VExpr → VExpr → VExpr → Prop wher
     Γ ⊢ e.inst e' : B.inst e' →
     Γ ⊢ .app (.lam A e) e' ≡ e.inst e' : B.inst e'
   | eta :
-    u.WF uvars → v.WF uvars → Γ ⊢ A : .sort u → A::Γ ⊢ B : .sort v →
+    u.WF uvars → v.WF uvars →
+    Γ ⊢ A : .sort u →
+    A::Γ ⊢ B : .sort v →
+    A.lift::A::Γ ⊢ B.liftN 1 1 : .sort v →
     Γ ⊢ e : .forallE A B →
+    A::Γ ⊢ e.lift : .forallE A.lift (B.liftN 1 1) →
     Γ ⊢ .lam A (.app e.lift (.bvar 0)) ≡ e : .forallE A B
   | proofIrrel :
     Γ ⊢ p : .sort .zero → Γ ⊢ h : p → Γ ⊢ h' : p →
@@ -65,6 +72,8 @@ inductive IsDefEqStrong : List VExpr → VExpr → VExpr → VExpr → Prop wher
     [] ⊢ df.type.instL ls : .sort u →
     [] ⊢ df.lhs.instL ls : df.type.instL ls →
     [] ⊢ df.rhs.instL ls : df.type.instL ls →
+    Γ ⊢ df.lhs.instL ls : df.type.instL ls →
+    Γ ⊢ df.rhs.instL ls : df.type.instL ls →
     Γ ⊢ df.lhs.instL ls ≡ df.rhs.instL ls : df.type.instL ls
 
 end
@@ -88,25 +97,32 @@ theorem IsDefEqStrong.weakN (W : Ctx.LiftN n k Γ Γ') (H : env.IsDefEqStrong U 
   | appDF h1 h2 _ _ _ _ _ ih1 ih2 ih3 ih4 ih5 =>
     refine liftN_inst_hi .. ▸ .appDF h1 h2 (ih1 W) (ih2 W.succ) (ih3 W) (ih4 W) ?_
     exact liftN_inst_hi .. ▸ liftN_inst_hi .. ▸ ih5 W
-  | lamDF h1 h2 _ _ _ ih1 ih2 ih3 => exact .lamDF h1 h2 (ih1 W) (ih2 W.succ) (ih3 W.succ)
-  | forallEDF h1 h2 _ _ ih1 ih2 => exact .forallEDF h1 h2 (ih1 W) (ih2 W.succ)
+  | lamDF h1 h2 _ _ _ _ _ ih1 ih2 ih3 ih4 ih5 =>
+    exact .lamDF h1 h2 (ih1 W) (ih2 W.succ) (ih3 W.succ) (ih4 W.succ) (ih5 W.succ)
+  | forallEDF h1 h2 _ _ _ ih1 ih2 ih3 => exact .forallEDF h1 h2 (ih1 W) (ih2 W.succ) (ih3 W.succ)
   | defeqDF h1 _ _ ih1 ih2 => exact .defeqDF h1 (ih1 W) (ih2 W)
   | beta h1 h2 _ _ _ _ _ _ ih1 ih2 ih3 ih4 ih5 ih6 =>
     refine liftN_inst_hi .. ▸ liftN_instN_hi .. ▸ .beta h1 h2
       (ih1 W) (ih2 W.succ) (ih3 W.succ) (ih4 W)
       (liftN_instN_hi .. ▸ ih5 W :)
       (liftN_instN_hi .. ▸ liftN_instN_hi .. ▸ ih6 W :)
-  | eta h1 h2 _ _ _ ih1 ih2 ih3 =>
-    have := IsDefEqStrong.eta h1 h2 (ih1 W) (ih2 W.succ) (ih3 W)
-    simp [liftN]; rwa [← lift_liftN']
+  | @eta Γ a u B v e h1 h2 _ _ _ _ _ ih1 ih2 ih3 ih4 ih5 =>
+    have := IsDefEqStrong.eta h1 h2 (ih1 W) (ih2 W.succ) ?_ (ih4 W) ?_
+    · simp [liftN]; rwa [← lift_liftN']
+    · specialize ih3 W.succ.succ
+      have := liftN'_comm B n 1 (k+1) 1 (Nat.le_add_left ..)
+      rw [Nat.add_comm 1] at this; rwa [← this, ← lift_liftN'] at ih3
+    · have ih5 : IsDefEqStrong _ _ _ _ _ (liftN n (lift (forallE ..)) _) := ih5 W.succ
+      rwa [← lift_liftN', ← lift_liftN'] at ih5
   | proofIrrel _ _ _ ih1 ih2 ih3 => exact .proofIrrel (ih1 W) (ih2 W) (ih3 W)
-  | extra h1 h2 h3 h4 h5 h6 h7 =>
+  | extra h1 h2 h3 h4 h5 h6 h7 _ _ _ _ _ ih4 ih5 =>
     have ⟨⟨hA1, _⟩, hA2, hA3⟩ := henv.closed.2 h1
-    rw [
+    specialize ih4 W; specialize ih5 W
+    simp [
       hA1.instL.liftN_eq (Nat.zero_le _),
       hA2.instL.liftN_eq (Nat.zero_le _),
-      hA3.instL.liftN_eq (Nat.zero_le _)]
-    exact .extra h1 h2 h3 h4 h5 h6 h7
+      hA3.instL.liftN_eq (Nat.zero_le _)] at ih4 ih5 ⊢
+    exact IsDefEqStrong.extra h1 h2 h3 h4 h5 h6 h7 ih4 ih5
 
 theorem IsDefEqStrong.defeq (H : IsDefEqStrong env U Γ e1 e2 A) : env.IsDefEq U Γ e1 e2 A := by
   induction H with
@@ -116,11 +132,11 @@ theorem IsDefEqStrong.defeq (H : IsDefEqStrong env U Γ e1 e2 A) : env.IsDefEq U
   | trans _ _ ih1 ih2 => exact .trans ih1 ih2
   | sortDF h1 h2 h3 => exact .sortDF h1 h2 h3
   | appDF _ _ _ _ _ _ _ _ _ ih1 ih2 => exact .appDF ih1 ih2
-  | lamDF _ _ _ _ _ ih1 _ ih2 => exact .lamDF ih1 ih2
-  | forallEDF _ _ _ _ ih1 ih2 => exact .forallEDF ih1 ih2
+  | lamDF _ _ _ _ _ _ _ ih1 _ _ ih2 => exact .lamDF ih1 ih2
+  | forallEDF _ _ _ _ _ ih1 ih2 => exact .forallEDF ih1 ih2
   | defeqDF _ _ _ ih1 ih2 => exact .defeqDF ih1 ih2
   | beta _ _ _ _ _ _ _ _ _ _ ih1 ih2 => exact .beta ih1 ih2
-  | eta _ _ _ _ _ _ _ ih => exact .eta ih
+  | eta _ _ _ _ _ _ _ _ _ _ ih => exact .eta ih
   | proofIrrel _ _ _ ih1 ih2 ih3 => exact .proofIrrel ih1 ih2 ih3
   | extra h1 h2 h3 => exact .extra h1 h2 h3
 
@@ -134,13 +150,14 @@ theorem IsDefEqStrong.mono
   | symm _ ih => exact .symm ih
   | trans _ _ ih1 ih2 => exact .trans ih1 ih2
   | appDF h1 h2 _ _ _ _ _ ih1 ih2 ih3 ih4 ih5 => exact .appDF h1 h2 ih1 ih2 ih3 ih4 ih5
-  | lamDF h1 h2  _ _ _ ih1 ih2 ih3 => exact .lamDF h1 h2 ih1 ih2 ih3
-  | forallEDF h1 h2 _ _ ih1 ih2 => exact .forallEDF h1 h2 ih1 ih2
+  | lamDF h1 h2  _ _ _ _ _ ih1 ih2 ih3 ih4 ih5 => exact .lamDF h1 h2 ih1 ih2 ih3 ih4 ih5
+  | forallEDF h1 h2 _ _ _ ih1 ih2 ih3 => exact .forallEDF h1 h2 ih1 ih2 ih3
   | defeqDF h1 _ _ ih1 ih2 => exact .defeqDF h1 ih1 ih2
   | beta h1 h2 _ _ _ _ _ _ ih1 ih2 ih3 ih4 ih5 ih6 => exact .beta h1 h2 ih1 ih2 ih3 ih4 ih5 ih6
-  | eta h1 h2 _ _ _ ih1 ih2 ih3 => exact .eta h1 h2 ih1 ih2 ih3
+  | eta h1 h2 _ _ _ _ _ ih1 ih2 ih3 ih4 ih5 => exact .eta h1 h2 ih1 ih2 ih3 ih4 ih5
   | proofIrrel _ _ _ ih1 ih2 ih3 => exact .proofIrrel ih1 ih2 ih3
-  | extra h1 h2 h3 h4 _ _ _ ih1 ih2 ih3 => exact .extra (henv.2 _ h1) h2 h3 h4 ih1 ih2 ih3
+  | extra h1 h2 h3 h4 _ _ _ _ _ ih1 ih2 ih3 ih4 ih5 =>
+    exact .extra (henv.2 _ h1) h2 h3 h4 ih1 ih2 ih3 ih4 ih5
 
 variable (henv : Ordered env) in
 theorem IsDefEqStrong.weak0 (H : env.IsDefEqStrong U [] e1 e2 A) :
@@ -165,22 +182,24 @@ theorem IsDefEqStrong.instL (H : env.IsDefEqStrong U Γ e1 e2 A) :
   | appDF _ _ _ _ _ _ _ ih1 ih2 ih3 ih4 ih5 =>
     exact instL_instN ▸ .appDF (.inst hls) (.inst hls)
       ih1 ih2 ih3 ih4 (instL_instN ▸ instL_instN ▸ ih5)
-  | lamDF _ _ _ _ _ ih1 ih2 ih3 =>
-    exact .lamDF (.inst hls) (.inst hls) ih1 ih2 ih3
-  | forallEDF _ _ _ _ ih1 ih2 =>
-    exact .forallEDF (.inst hls) (.inst hls) ih1 ih2
+  | lamDF _ _ _ _ _ _ _ ih1 ih2 ih3 ih4 ih5 =>
+    exact .lamDF (.inst hls) (.inst hls) ih1 ih2 ih3 ih4 ih5
+  | forallEDF _ _ _ _ _ ih1 ih2 ih3 =>
+    exact .forallEDF (.inst hls) (.inst hls) ih1 ih2 ih3
   | defeqDF _ _ _ ih1 ih2 =>
     exact .defeqDF (.inst hls) ih1 ih2
   | beta _ _ _ _ _ _ _ _ ih1 ih2 ih3 ih4 ih5 ih6 =>
     simpa using .beta (.inst hls) (.inst hls) ih1 ih2 ih3 ih4
       (by simpa using ih5) (by simpa using ih6)
-  | eta _ _ _ _ _ ih1 ih2 ih3 =>
-    simpa [VExpr.instL] using .eta (.inst hls) (.inst hls) ih1 ih2 ih3
+  | eta _ _ _ _ _ _ _ ih1 ih2 ih3 ih4 ih5 =>
+    simpa [VExpr.instL] using .eta (.inst hls) (.inst hls) ih1 ih2
+      (by simpa using ih3) ih4 (by simpa [VExpr.instL] using ih5)
   | proofIrrel _ _ _ ih1 ih2 ih3 =>
     exact .proofIrrel ih1 ih2 ih3
-  | extra h1 h2 h3 _ _ _ _ ih1 ih2 ih3 =>
-    simp [VExpr.instL, VExpr.instL_instL] at ih1 ih2 ih3 ⊢
-    exact .extra h1 (by simp [h2, VLevel.WF.inst hls]) (by simp [h3]) (.inst hls) ih1 ih2 ih3
+  | extra h1 h2 h3 _ _ _ _ _ _ ih1 ih2 ih3 ih4 ih5 =>
+    simp [VExpr.instL, VExpr.instL_instL] at ih1 ih2 ih3 ih4 ih5 ⊢
+    exact .extra h1 (by simp [h2, VLevel.WF.inst hls]) (by simp [h3])
+      (.inst hls) ih1 ih2 ih3 ih4 ih5
 
 def CtxStrong (env : VEnv) (U Γ) :=
   OnCtx Γ fun Γ A => ∃ u, env.IsDefEqStrong U Γ A A (.sort u)
@@ -223,12 +242,14 @@ theorem IsDefEqStrong.instN (W : Ctx.InstN Γ₀ e₀ A₀ k Γ₁ Γ) (H : env.
     exact inst0_inst_hi .. ▸ .appDF h1 h2
       (ih1 W hΓ) (ih2 W.succ ⟨hΓ, _, ih1 W hΓ⟩)
       (ih3 W hΓ) (ih4 W hΓ) (inst0_inst_hi .. ▸ inst0_inst_hi .. ▸ ih5 W hΓ)
-  | lamDF h1 h2 _ _ _ ih1 ih2 ih3 =>
+  | lamDF h1 h2 _ _ _ _ _ ih1 ih2 ih3 ih4 ih5 =>
     exact
       have hΓ' := ⟨hΓ, _, (ih1 W hΓ).hasType.1⟩
-      .lamDF h1 h2 (ih1 W hΓ) (ih2 W.succ hΓ') (ih3 W.succ hΓ')
-  | forallEDF h1 h2 _ _ ih1 ih2 =>
-    exact .forallEDF h1 h2 (ih1 W hΓ) (ih2 W.succ ⟨hΓ, _, (ih1 W hΓ).hasType.1⟩)
+      have hΓ'' := ⟨hΓ, _, (ih1 W hΓ).hasType.2⟩
+      .lamDF h1 h2 (ih1 W hΓ) (ih2 W.succ hΓ') (ih3 W.succ hΓ'') (ih4 W.succ hΓ') (ih5 W.succ hΓ'')
+  | forallEDF h1 h2 _ _ _ ih1 ih2 ih3 =>
+    exact .forallEDF h1 h2 (ih1 W hΓ)
+      (ih2 W.succ ⟨hΓ, _, (ih1 W hΓ).hasType.1⟩) (ih3 W.succ ⟨hΓ, _, (ih1 W hΓ).hasType.2⟩)
   | defeqDF h1 _ _ ih1 ih2 => exact .defeqDF h1 (ih1 W hΓ) (ih2 W hΓ)
   | beta h1 h2 _ _ _ _ _ _ ih1 ih2 ih3 ih4 ih5 ih6 =>
     rw [inst0_inst_hi, inst0_inst_hi]; exact
@@ -236,20 +257,30 @@ theorem IsDefEqStrong.instN (W : Ctx.InstN Γ₀ e₀ A₀ k Γ₁ Γ) (H : env.
       .beta h1 h2
         (ih1 W hΓ) (ih2 W.succ hΓ') (ih3 W.succ hΓ') (ih4 W hΓ)
         (inst0_inst_hi .. ▸ ih5 W hΓ) (inst0_inst_hi .. ▸ inst0_inst_hi .. ▸ ih6 W hΓ)
-  | eta h1 h2 _ _ _ ih1 ih2 ih3 =>
+  | eta h1 h2 _ _ _ _ _ ih1 ih2 ih3 ih4 ih5 =>
     have :=
       have hΓ' := ⟨hΓ, _, (ih1 W hΓ).hasType.1⟩
-      IsDefEqStrong.eta h1 h2 (ih1 W hΓ) (ih2 W.succ hΓ') (ih3 W hΓ)
+      IsDefEqStrong.eta h1 h2 (ih1 W hΓ) (ih2 W.succ hΓ')
+        (by
+          have := ih3 W.succ.succ ⟨hΓ', _, by
+            rw [← lift_instN_lo]; exact (ih1 W hΓ).hasType.1.weakN henv .one⟩
+          rwa [lift_instN_lo, liftN_instN_lo (hj := Nat.le_add_left ..), Nat.add_comm 1])
+        (ih4 W hΓ)
+        (by
+          have := ih5 W.succ hΓ'
+          simp only [inst, ← lift_instN_lo] at this
+          rwa [liftN_instN_lo (hj := Nat.le_add_left ..), Nat.add_comm 1])
     rw [lift, liftN_instN_lo (hj := Nat.zero_le _), Nat.add_comm] at this
     simpa [inst]
   | proofIrrel _ _ _ ih1 ih2 ih3 => exact .proofIrrel (ih1 W hΓ) (ih2 W hΓ) (ih3 W hΓ)
-  | extra h1 h2 h3 h4 h5 h6 h7 =>
+  | extra h1 h2 h3 h4 h5 h6 h7 _ _ _ _ _ ih4 ih5 =>
     have ⟨⟨hA1, _⟩, hA2, hA3⟩ := henv.closed.2 h1
-    rw [
+    specialize ih4 W hΓ; specialize ih5 W hΓ
+    simp [
       hA1.instL.instN_eq (Nat.zero_le _),
       hA2.instL.instN_eq (Nat.zero_le _),
-      hA3.instL.instN_eq (Nat.zero_le _)]
-    exact .extra h1 h2 h3 h4 h5 h6 h7
+      hA3.instL.instN_eq (Nat.zero_le _)] at ih4 ih5 ⊢
+    exact .extra h1 h2 h3 h4 h5 h6 h7 ih4 ih5
 
 theorem IsDefEqStrong.defeqDF_l (henv : Ordered env) (hΓ : CtxStrong env U Γ)
     (h1 : env.IsDefEqStrong U Γ A A' (.sort u))
@@ -261,10 +292,10 @@ theorem IsDefEqStrong.defeqDF_l (henv : Ordered env) (hΓ : CtxStrong env U Γ)
       |>.symm.defeqDF hu (.bvar .zero hu (h1.hasType.2.weakN henv .one))
       |>.instN henv hΓ' .zero (h2.weakN henv (.succ (.one (A := A')))) hΓ'
 
-structure EnvStrong (env : VEnv) (U : Nat) (e A : VExpr) : Prop where
-  val : env.IsDefEqStrong U [] e e A
-  type : ∃ u, env.IsDefEqStrong U [] A A (.sort u)
-  forallE_inv : ∀ A B, e = A.forallE B →
+def EnvStrong (env : VEnv) (U : Nat) (e A : VExpr) : Prop :=
+  env.IsDefEqStrong U [] e e A ∧
+  (∃ u, env.IsDefEqStrong U [] A A (.sort u)) ∧
+  ∀ A B, e = A.forallE B →
     (∃ u, env.IsDefEqStrong U [] A A (.sort u)) ∧
     (∃ u, env.IsDefEqStrong U [A] B B (.sort u))
 
@@ -296,7 +327,7 @@ theorem IsDefEqStrong.forallE_inv' (hΓ : CtxStrong env U Γ)
       refine ⟨⟨_, h4.instN henv hΓ .zero A1 hΓ⟩, _, h4.instN henv hΓ (.succ .zero) A2 ?_⟩
       exact ⟨hΓ, _, h4.instN henv hΓ .zero A1 hΓ⟩
     | _ => cases eq
-  | eta _ _ _ _ _ _ _ ih =>
+  | eta _ _ _ _ _ _ _ _ _ _ ih =>
     obtain ⟨⟨⟩⟩ | eq := eq
     exact ih hΓ (.inl eq)
   | @extra df ls _ Γ h1 h2 =>
@@ -308,7 +339,7 @@ theorem IsDefEqStrong.forallE_inv' (hΓ : CtxStrong env U Γ)
       cases eq <;> exact this _ ‹_› ‹_›
     intro e eq IH
     cases e <;> cases eq; rename_i A B
-    let ⟨⟨_, A1⟩, v, A2⟩ := IH.forallE_inv _ _ rfl
+    let ⟨⟨_, A1⟩, v, A2⟩ := IH.2.2 _ _ rfl
     refine ⟨⟨_, (A1.instL h2).weak0 henv⟩, v.inst ls, ?_⟩
     have := (A2.instL h2).weakN henv (.succ (.zero Γ))
     have C1 := (A1.instL h2).defeq.closedN henv ⟨⟩
@@ -324,10 +355,10 @@ theorem IsDefEqStrong.isType' (hΓ : CtxStrong env U Γ) (H : env.IsDefEqStrong 
   | bvar h => exact hΓ.lookup henv h
   | const h1 h2 =>
     let ⟨_, h⟩ := envIH.1 h1
-    exact ⟨_, (h.val.instL h2).weak0 henv⟩
+    exact ⟨_, (h.1.instL h2).weak0 henv⟩
   | proofIrrel h1 => exact ⟨_, h1⟩
   | extra h1 h2 =>
-    have ⟨_, h⟩ := (envIH.2 h1).2.type
+    have ⟨_, h⟩ := (envIH.2 h1).2.2.1
     exact ⟨_, (h.instL h2).weak0 henv⟩
   | sortDF h1 => exact ⟨_, .sortDF h1 h1 rfl⟩
   | symm _ ih => exact ih hΓ
@@ -336,11 +367,11 @@ theorem IsDefEqStrong.isType' (hΓ : CtxStrong env U Γ) (H : env.IsDefEqStrong 
     let ⟨_, ih3⟩ := ih3 hΓ
     have ⟨_, _, ih3⟩ := ih3.forallE_inv' henv envIH hΓ (.inl rfl)
     exact ⟨_, h4.hasType.1.instN henv hΓ .zero ih3 hΓ⟩
-  | lamDF h1 h2 h3 h4 => exact ⟨_, .forallEDF h1 h2 h3.hasType.1 h4⟩
+  | lamDF h1 h2 h3 h4 => exact ⟨_, .forallEDF h1 h2 h3.hasType.1 h4 h4⟩
   | forallEDF h1 h2 => exact ⟨_, .sortDF ⟨h1, h2⟩ ⟨h1, h2⟩ rfl⟩
   | defeqDF _ h2 => exact ⟨_, h2.hasType.2⟩
   | beta _ _ _ h4 _ h6 => exact ⟨_, h6.hasType.1.instN henv hΓ .zero h4 hΓ⟩
-  | eta _ _ _ _ _ _ _ ih => exact ih hΓ
+  | eta _ _ _ _ _ _ _ _ _ _ ih => exact ih hΓ
 
 theorem IsDefEqStrong.instDF
     (henv : Ordered env) (hΓ : CtxStrong env U Γ) (hu : u.WF U) (hv : v.WF U)
@@ -363,7 +394,7 @@ theorem IsDefEqStrong.instDF
         (ha.hasType.1.instN henv hΓ .zero hB hΓ)
         (ha.hasType.1.instN henv hΓ .zero hf.hasType.1 hΓ)
     (H1 hf ha.hasType.1).symm.trans <|
-      .trans (.appDF hu hv hA hB (.lamDF hu hv hA hB hf) ha hi) <|
+      .trans (.appDF hu hv hA hB (.lamDF hu hv hA hB hB hf hf) ha hi) <|
       .defeqDF hv (.symm hi) (H1 hf.hasType.2 ha.hasType.2)
   H2 hv hB hf <| H2 (v := v.succ) hv (.sortDF hv hv rfl) hB (.sortDF hv hv rfl)
 
@@ -378,7 +409,7 @@ theorem IsDefEq.strong' (hΓ : CtxStrong env U Γ)
     exact .bvar h (hA.defeq.sort_r henv (hctx hΓ)) hA
   | @const _ _ ls' _ h1 h2 h3 =>
     let ⟨u, h4⟩ := envIH.1 h1
-    exact .const h1 h2 h3 (.inst h2) (h4.val.instL h2)
+    exact .const h1 h2 h3 (.inst h2) (h4.1.instL h2)
   | symm _ ih => exact (ih hΓ).symm
   | trans _ _ ih1 ih2 => exact (ih1 hΓ).trans (ih2 hΓ)
   | sortDF h1 h2 h3 => exact .sortDF h1 h2 h3
@@ -394,11 +425,13 @@ theorem IsDefEq.strong' (hΓ : CtxStrong env U Γ)
     have hu := hA.sort_r henv hΓ.defeq
     have hΓ' : CtxStrong env U (_::_) := ⟨hΓ, _, (ih1 hΓ).hasType.1⟩
     let ⟨_, hB⟩ := (ih2 hΓ').isType' henv envIH hΓ'
-    exact .lamDF hu (hB.defeq.sort_r henv hΓ'.defeq) (ih1 hΓ) hB (ih2 hΓ')
+    exact .lamDF hu (hB.defeq.sort_r henv hΓ'.defeq) (ih1 hΓ)
+      hB ((ih1 hΓ).defeqDF_l henv hΓ hB) (ih2 hΓ') ((ih1 hΓ).defeqDF_l henv hΓ (ih2 hΓ'))
   | forallEDF hA hb ih1 ih2 =>
     have hu := hA.sort_r henv hΓ.defeq
     have hΓ' : CtxStrong env U (_::_) := ⟨hΓ, _, (ih1 hΓ).hasType.1⟩
-    exact .forallEDF hu (hb.sort_r henv hΓ'.defeq) (ih1 hΓ) (ih2 hΓ')
+    exact .forallEDF hu (hb.sort_r henv hΓ'.defeq)
+      (ih1 hΓ) (ih2 hΓ') ((ih1 hΓ).defeqDF_l henv hΓ (ih2 hΓ'))
   | defeqDF hAB _ ih1 ih2 =>
     exact .defeqDF (hAB.sort_r henv hΓ.defeq) (ih1 hΓ) (ih2 hΓ)
   | beta _ _ ih1 ih2 =>
@@ -414,24 +447,31 @@ theorem IsDefEq.strong' (hΓ : CtxStrong env U Γ)
     let ⟨_, hAB⟩ := he.isType' henv envIH hΓ
     let ⟨⟨u, hA⟩, ⟨v, hB⟩⟩ := hAB.forallE_inv' henv envIH hΓ (.inl rfl)
     have hΓ' : CtxStrong env U (_::_) := ⟨hΓ, _, hA⟩
-    exact .eta (hA.defeq.sort_r henv hΓ.defeq) (hB.defeq.sort_r henv hΓ'.defeq) hA hB he
+    exact .eta (hA.defeq.sort_r henv hΓ.defeq) (hB.defeq.sort_r henv hΓ'.defeq)
+      hA hB (hB.weakN henv (.succ .one)) he (he.weakN henv .one)
   | proofIrrel _ _ _ ih1 ih2 ih3 => exact .proofIrrel (ih1 hΓ) (ih2 hΓ) (ih3 hΓ)
   | extra h1 h2 h3 =>
     let ⟨⟨hl, ⟨_, ht⟩, _⟩, hr, _, _⟩ := envIH.2 h1
-    exact .extra h1 h2 h3 (.inst h2) (ht.instL h2) (hl.instL h2) (hr.instL h2)
+    exact .extra h1 h2 h3 (.inst h2) (ht.instL h2)
+      (hl.instL h2) (hr.instL h2) ((hl.instL h2).weak0 henv) ((hr.instL h2).weak0 henv)
 
-variable (henv : Ordered env) (envIH : env.OnTypes (EnvStrong env)) in
-theorem CtxStrong.strong (hΓ : OnCtx Γ (env.IsType U)) : CtxStrong env U Γ := by
+theorem CtxStrong.strong' (henv : Ordered env) (envIH : env.OnTypes (EnvStrong env))
+    (hΓ : OnCtx Γ (env.IsType U)) : CtxStrong env U Γ := by
   induction Γ with
   | nil => trivial
   | cons _ _ ih => let ⟨hΓ, _, hA⟩ := hΓ; exact ⟨ih hΓ, _, hA.strong' henv envIH (ih hΓ)⟩
 
-theorem IsDefEq.strong (henv : Ordered env) (hΓ : OnCtx Γ (env.IsType U))
-    (H : env.IsDefEq U Γ e1 e2 A) : env.IsDefEqStrong U Γ e1 e2 A := by
-  refine H.strong' henv ?a (.strong henv ?a hΓ)
-  exact henv.induction _
-    (fun le ⟨h1, ⟨_, h2⟩, h3⟩ => ⟨h1.mono le, ⟨_, h2.mono le⟩, fun A B eq =>
+theorem Ordered.strong (henv : Ordered env) : OnTypes env (EnvStrong env) :=
+  henv.induction _
+    (fun le ⟨h1, ⟨_, h2⟩, h3⟩ => ⟨h1.mono le, ⟨_, h2.mono le⟩, fun _ _ eq =>
       let ⟨⟨_, h4⟩, ⟨_, h5⟩⟩ := h3 _ _ eq; ⟨⟨_, h4.mono le⟩, ⟨_, h5.mono le⟩⟩⟩)
     (fun henv IH H =>
       have H' := H.strong' henv IH (Γ := []) ⟨⟩
       ⟨H', H'.isType' henv IH ⟨⟩, fun _ _ eq => H'.forallE_inv' henv IH ⟨⟩ (.inl eq)⟩)
+
+theorem CtxStrong.strong (henv : Ordered env) (hΓ : OnCtx Γ (env.IsType U)) : CtxStrong env U Γ :=
+  .strong' henv henv.strong hΓ
+
+theorem IsDefEq.strong (henv : Ordered env) (hΓ : OnCtx Γ (env.IsType U))
+    (H : env.IsDefEq U Γ e1 e2 A) : env.IsDefEqStrong U Γ e1 e2 A :=
+  H.strong' henv henv.strong (.strong henv hΓ)
